Java/src/Java/Func/Reify.v
@@ -90,7 +90,20 @@ Ltac reify_typ e :=
              [[ (fun (y : @mk_dvar_map _ _ _ _ term_table elem_ctor) => True) ]]
              [[ e ]].
 
-Goal (forall (Pr : Program) (C : class) (v : val) (x f : String.string) (fields : list field) (ex : @Open.expr Lang.var val), True).
+Notation "'ap_eq' '[' x ',' y ']'" :=
+	 (ap (T := RFun (RFun String.string val)) (ap (T := RFun (RFun String.string val)) (pure (T := RFun (RFun String.string val)) (@eq val)) x) y).
+Notation "'ap_pointsto' '[' x ',' f ',' e ']'" :=
+	(ap (T := RFun (RFun String.string val)) (ap (T := RFun (RFun String.string val)) (ap (T := RFun (RFun String.string val))
+		(pure (T := RFun (RFun String.string val)) pointsto) (stack_get x))
+			(pure (T := RFun (RFun String.string val)) f)) e).
+Notation "'ap_typeof' '[' e ',' C ']'" :=
+	(ap (T := RFun (RFun String.string val))
+	    (ap (T := RFun (RFun String.string val))
+	        (pure (T := RFun (RFun String.string val)) typeof)
+	        (pure (T := RFun (RFun String.string val)) C))
+	    e).
+
+Goal (forall (Pr : Program) (C : class) (v : val) (x f : String.string) (fields : list field) (ex : (RFun (RFun String.string val) val)), True).
   intros Pr C v x f fields ex.
   reify_java 5.
   reify_java (typeof C v).
@@ -106,7 +119,7 @@ Goal (forall (Pr : Program) (C : class) (v : val) (x f : String.string) (fields 
   reify_java (exists x, x = 5).
   reify_java (forall x, x = 5).
 
-  reify_java (pure (T := RFun (RFun String.string val)) pointsto).
+  reify_java (ap (T := RFun (RFun String.string val)) (ap (T := RFun (RFun String.string val)) (pure (T := RFun (RFun String.string val)) pointsto) (stack_get x)) (pure (T := RFun (RFun String.string val)) x)).
 
   reify_java (fun a b c => pointsto a b c).
 
@@ -116,14 +129,15 @@ Goal (forall (Pr : Program) (C : class) (v : val) (x f : String.string) (fields 
   reify_java (pure (T := RFun (RFun String.string val)) (vbool true)).
 
   reify_java (forall x : nat, x = x).
-  reify_java (exists x : Lang.stack, True).
+Check @pure.
   reify_java (ap (T := RFun (RFun String.string val)) (pure (T := RFun (RFun String.string val)) (@eq val)) (eval d)).
 
-  reify_java ((ap (ap (T := Fun Lang.stack) (pure (T := Fun Lang.stack) (@eq val)) (eval d)) (pure (vbool true)))).
+  reify_java (ap_pointsto [x, x, (eval d)]).
 
   generalize String.EmptyString. intro c.
   reify_java (cread c c c).
 
+   reify_java (ltrue |-- triple ltrue ltrue (cread c c c)).
    reify_java (ltrue |-- {[ ltrue ]} cread c c c {[ ltrue ]}).
 
   reify_java cskip.
@@ -133,7 +147,7 @@ Goal (forall (Pr : Program) (C : class) (v : val) (x f : String.string) (fields 
   reify_java (forall x : nat, x = x).
   reify_java (exists x : nat, x = x).
 
-  reify_java (@subst1 Lang.var val _).
+  reify_java (@subst1 String.string val _).
   reify_java (cseq cskip cskip).
 
   reify_java (@map nat nat).
@@ -147,8 +161,8 @@ Goal (forall (Pr : Program) (C : class) (v : val) (x f : String.string) (fields 
   generalize (String.EmptyString : String.string).
   intro y.
 
-  reify_java (stack_get (A := Lang.var) (val := val)).
-  reify_java (@stack_get Lang.var val y).
+  reify_java (stack_get (A := String.string) (val := val)).
+  reify_java (@stack_get String.string val y).
 
   reify_java (stack_get (val := val) y).
 
@@ -159,325 +173,3 @@ Goal (forall (Pr : Program) (C : class) (v : val) (x f : String.string) (fields 
   exact I.
 
 Defined.
-
-
-
-Ltac reify trm :=
-  let t := fresh "t" in
-  let k e := pose e as t
-  in
-  reify_expr reify_typ k [[ True ]] [[ trm ]]; cbv beta iota in t.
-
-Goal True.
-  reify nat.
-  reify bool.
-  reify String.string.
-  reify (list bool).
-  reify (list (list (list (spec * list ((stack String.string val -> asn)))))).
-  unfold typ2, Typ2_tyArr, Typ2_Fun, typ0, Typ0_tyString, Typ0_tyVal, Typ0_sym in t3.
-Abort.
-
-Reify Declare Patterns patterns_java_typ : typ.
-
-Reify Declare Patterns patterns_java : (ExprCore.expr typ func).
-
-Local Instance Applicative_Fun A : Applicative (RFun A) :=
-{ pure := fun _ x _ => x
-; ap := fun _ _ f x y => (f y) (x y)
-}.
-
-(*
-Reify Declare Patterns const_for_cmd += ((RHasType cmd ?0) => (fun (c : id cmd) => mkCmd [c] : expr typ func)).
-*)
-
-(* Axiom t : Type. *)
-(* Reify Declare Patterns t_pat : t. *)
-
-(* Reify Declare Syntax t_cmd := (@Patterns.CPatterns t t_pat). *)
-
-Reify Declare Syntax reify_imp_typ :=
-  (@Patterns.CFix@{Set} _
-      (@Patterns.CFirst_@{Set} _
-         ((@Patterns.CPatterns@{Set} typ patterns_java_typ) ::
-          (@CPattern@{Set} _ (_ :: _ :: nil)
-                     (@RImpl (RGet 0 RIgnore) (RGet 1 RIgnore))
-                     (fun (a b : function (CRec 0)) => tyArr a b)) :: nil))).
-
-Reify Declare Typed Table term_table : BinNums.positive => typ.
-
-Require Import MirrorCore.ExprI.
-Require Import ExtLib.Data.SumN.
-Import OneOfType.
-Let Ext (x : SymEnv.func) := @ExprCore.Inj typ func (Into (ts := func_map) 2 eq_refl x).
-
-Reify Declare Syntax reify_imp :=
-  @Patterns.CFix@{Set} (expr typ func)
-    (@Patterns.CFirst_@{Set} _
-       ((Patterns.CVar@{Set} (@ExprCore.Var typ func)) ::
-        (Patterns.CPatterns@{Set} patterns_java) ::
-        (Patterns.CApp@{Set Set Set} (Patterns.CRec@{Set} 0) (Patterns.CRec@{Set} 0) (@ExprCore.App typ func)) ::
-	(Patterns.CAbs@{Set Set Set} (CCall@{Set} reify_imp_typ) (CRec@{Set} 0) (@ExprCore.Abs typ func)) ::
-	(Patterns.CMap@{Set Set} Ext (Patterns.CTypedTable@{Set Set} reify_imp_typ term_table) :: nil))).
-
-Notation "'ap_eq' '[' x ',' y ']'" :=
-	 (ap (T := Fun Lang.stack) (ap (T := Fun Lang.stack) (pure (T := Fun Lang.stack) (@eq val)) x) y).
-Notation "'ap_pointsto' '[' x ',' f ',' e ']'" :=
-	(ap (T := Fun Lang.stack) (ap (T := Fun Lang.stack) (ap (T := Fun Lang.stack)
-		(pure (T := Fun Lang.stack) pointsto) (stack_get x))
-			(pure (T := Fun Lang.stack) f)) e).
-Notation "'ap_typeof' '[' e ',' C ']'" :=
-	(ap (T := Fun Lang.stack)
-	    (ap (T := Fun Lang.stack)
-	        (pure (T := Fun Lang.stack) typeof)
-	        (pure (T := Fun Lang.stack) C))
-	    e).
-(*
-Definition set_fold_fun (x f : String.string) (P : sasn) :=
-	ap_pointsto [x, f, pure null] ** P.
-*)
-Let _Inj := @ExprCore.Inj typ func.
-
-(*
-Reify Seed Typed Table term_table += 1 => [ (tyArr tyVal (tyArr (tyList tyVal) tyAsn)) , List ].
-Reify Seed Typed Table term_table += 2 => [ (tyArr tyVal (tyArr (tyList tyVal) tyAsn)) , NodeList ].
-*)
-
-Local Notation "x @ y" := (@RApp x y) (only parsing, at level 30).
-Local Notation "'!!' x" := (@RExact _ x) (only parsing, at level 25).
-Local Notation "'?' n" := (@RGet n RIgnore) (only parsing, at level 25).
-Local Notation "'?!' n" := (@RGet n RConst) (only parsing, at level 25).
-Local Notation "'#'" := RIgnore (only parsing, at level 0).
-
-Print function.
-About reify_imp_typ.
-
-Reify Pattern patterns_java += (RPi (?0) (?1)) =>
-  (fun (x : function@{Set} (CCall@{Set} reify_imp_typ)) (y : function (CCall reify_imp)) =>
-     ExprCore.App (Inj (fForall (func := func) x tyProp)) (ExprCore.Abs x y)).
-
-
-(* This is now embedded inside the reification system. *)
-(* Reify Pattern patterns_java_typ += (@RImpl (RGet 0 RIgnore) (RGet 1 RIgnore)) => *)
-(*     (fun (a b : function reify_imp_typ) => tyArr a b). *)
-
-Reify Pattern patterns_java_typ += (!! asn)  => tyAsn.
-Reify Pattern patterns_java_typ += (!! sasn) => tySasn.
-Reify Pattern patterns_java_typ += (!! (@vlogic Lang.var val)) => tyPure.
-Reify Pattern patterns_java_typ += (!! Prop) => tyProp.
-Reify Pattern patterns_java_typ += (!! spec) => tySpec.
-
-Reify Pattern patterns_java_typ += (!! @prod @ ?0 @ ?1) =>
-   (fun (x y : function (CCall reify_imp_typ)) => tyProd x y).
-Reify Pattern patterns_java_typ += (!! (@list String.string)) => tyStringList.
-Reify Pattern patterns_java_typ += (!! (@list field)) => tyFields.
-Reify Pattern patterns_java_typ += (!! (@list (@Open.expr (Lang.var) val))) => tyStringList.
-Reify Pattern patterns_java_typ += (!! (@list (Lang.var * @Open.expr (Lang.var) val))) => tySubstList.
-Reify Pattern patterns_java_typ += (!! (@substlist Lang.var val)) => tySubstList.
-Reify Pattern patterns_java_typ += (!! @list @ ?0) =>
-   (fun x : function (CCall reify_imp_typ) => tyList x).
-Reify Pattern patterns_java_typ += (!! nat) => tyNat.
-Reify Pattern patterns_java_typ += (!! val) => tyVal.
-Reify Pattern patterns_java_typ += (!! bool) => tyBool.
-Reify Pattern patterns_java_typ += (!! field) => tyString.
-Reify Pattern patterns_java_typ += (!! class) => tyString.
-Reify Pattern patterns_java_typ += (!! @Open.open Lang.var val asn) => tySasn.
-Reify Pattern patterns_java_typ += (!! @Open.open Lang.var val Prop) => tyPure.
-Reify Pattern patterns_java_typ += (!! Lang.var) => tyString.
-Reify Pattern patterns_java_typ += (!! String.string) => tyString.
-Reify Pattern patterns_java_typ += (!! Program) => tyProg.
-Reify Pattern patterns_java_typ += (!! Lang.stack) => tyStack.
-Reify Pattern patterns_java_typ += (!! @Stack.stack Lang.var val) => tyStack.
-Reify Pattern patterns_java_typ += (!! cmd) => tyCmd.
-Reify Pattern patterns_java_typ += (!! dexpr) => tyDExpr.
-Reify Pattern patterns_java_typ += (!! (@Open.expr Lang.var val)) => tyExpr.
-(* Reify Pattern patterns_java_typ += (!! @Subst.subst (String.string) val) => tySubst. *) (** TODO: Commented *)
-
-(** TODO(gmalecha): This should be moved up *)
-Reify Pattern patterns_java_typ += (!! Fun @ ?0 @ ?1) =>
-  (fun (a b : function (CCall reify_imp_typ)) => tyArr a b).
-
-Reify Pattern patterns_java += (RHasType String.string (?0)) => (fun (s : id String.string) => mkString (func := func) (typ := typ) s).
-Reify Pattern patterns_java += (RHasType field (?0)) => (fun (f : id field) => mkString (typ := typ) (func := func) f).
-Reify Pattern patterns_java += (RHasType Lang.var (?0)) => (fun (f : id Lang.var) => mkString (typ := typ) (func := func) f).
-Reify Pattern patterns_java += (RHasType val (?0)) => (fun (v : id val) => Inj (typ := typ) (fVal v)).
-Reify Pattern patterns_java += (RHasType bool (?0)) => (fun (b : id bool) => mkBool (typ := typ) (func := func) b).
-Reify Pattern patterns_java += (RHasType nat (?0)) => (fun (n : id nat) => mkNat (typ := typ) (func := func) n).
-Reify Pattern patterns_java += (RHasType cmd (?0)) => (fun (c : id cmd) => Inj (typ := typ) (fCmd c)).
-Reify Pattern patterns_java += (RHasType dexpr (?0)) => (fun (e : id dexpr) => Inj (typ := typ) (fDExpr e)).
-Reify Pattern patterns_java += (RHasType Program (?0)) => (fun (P : id Program) => (Inj (typ := typ) (fProg P))).
-Reify Pattern patterns_java += (RHasType (list field) (?0)) => (fun (fs : id (list field)) => Inj (typ := typ) (fFields fs)).
-Reify Pattern patterns_java += (RHasType class (?0)) => (fun (c : id class) => mkString (typ := typ) (func := func) c).
-
-Reify Pattern patterns_java += (RHasType (@list dexpr) (?0)) => (fun (es : id (@list dexpr)) => mkExprList es).
-Reify Pattern patterns_java += (RHasType (@list String.string) (?0)) => (fun (vs : id (@list String.string)) => Inj (typ := typ) (fFields vs)).
-Reify Pattern patterns_java += (!! (@eq) @ ?0) =>
-  (fun (x : function (CCall reify_imp_typ)) => Inj (typ := typ) (fEq (func := func) x)).
-
-(** Intuitionistic Operators **)
-Reify Pattern patterns_java += (!! @ILogic.lentails @ ?0 @ #) =>
-  (fun (x : function (CCall reify_imp_typ)) => Inj (typ := typ) (fEntails x)).
-Reify Pattern patterns_java += (!! @ILogic.ltrue @ ?0 @ #) =>
-  (fun (x : function (CCall reify_imp_typ)) => mkTrue (func := func) x).
-Reify Pattern patterns_java += (!! @ILogic.lfalse @ ?0 @ #) =>
-  (fun (x : function (CCall reify_imp_typ)) => mkFalse (func := func) x).
-
-Reify Pattern patterns_java += (!! @ILogic.land @ ?0 @ #) =>
-  (fun (x : function (CCall reify_imp_typ)) => Inj (typ := typ) (fAnd (func := func) x)).
-Reify Pattern patterns_java += (!! @ILogic.lor @ ?0 @ #) => (fun (x : function (CCall reify_imp_typ)) => Inj (typ := typ) (fOr (func := func) x)).
-Reify Pattern patterns_java += (!! @ILogic.limpl @ ?0 @ #) => (fun (x : function (CCall reify_imp_typ)) => Inj (typ := typ) (fImpl (func := func) x)).
-
-Reify Pattern patterns_java += (!! @ILogic.lexists @ ?0 @ # @ ?1) => (fun (x y : function (CCall reify_imp_typ)) => Inj (typ := typ) (fExists (func := func) y x)).
-
-Reify Pattern patterns_java += (!! @ILogic.lforall @ ?0 @ # @ ?1) => (fun (x y : function (CCall reify_imp_typ)) => Inj (typ := typ) (fForall (func := func) y x)).
-(** Embedding Operators **)
-Reify Pattern patterns_java += (!! @ILEmbed.embed @ ?0 @ ?1 @ #) => (fun (x y : function (CCall reify_imp_typ)) => Inj (typ := typ) (fEmbed (func := func) x y)).
-
-Reify Pattern patterns_java += (!! @pair @ ?0 @ ?1) => (fun (x y : function (CCall reify_imp_typ)) => Inj (typ := typ) (fPair (func := func) x y)).
-
-(** Special cases for Coq's primitives **)
-Reify Pattern patterns_java += (!! True) => (mkTrue (func := func) tyProp).
-Reify Pattern patterns_java += (!! False) => (mkFalse (func := func) tyProp).
-Reify Pattern patterns_java += (!! and) => (Inj (typ := typ) (fAnd (func := func) tyProp)).
-
-Reify Pattern patterns_java += (!! or) => (Inj (typ := typ) (fOr (func := func) tyProp)).
-
-Reify Pattern patterns_java += (!! ex @ ?0) => (fun (x : function (CCall reify_imp_typ)) => Inj (typ := typ) (fExists (func := func) x tyProp)).
-
-Reify Pattern patterns_java += (RPi (?0) (?1)) =>
-  (fun (x : function (CCall reify_imp_typ)) (y : function (CCall reify_imp)) =>
-     ExprCore.App (Inj (fForall (func := func) x tyProp)) (ExprCore.Abs x y)).
-
-Reify Pattern patterns_java += (RImpl (?0) (?1)) => (fun (x y : function (CCall reify_imp)) =>
-	ExprCore.App (ExprCore.App (Inj (fImpl (func := func) tyProp)) x) y).
-
-(** Separation Logic Operators **)
-Reify Pattern patterns_java += (!! @BILogic.sepSP @ ?0 @ #) => (fun (x : function (CCall reify_imp_typ)) => Inj (typ := typ) (fStar (func := func) x)).
-Reify Pattern patterns_java += (!! @BILogic.wandSP @ ?0 @ #) => (fun (x : function (CCall reify_imp_typ)) => Inj (typ := typ) (fWand (func := func) x)).
-Reify Pattern patterns_java += (!! @BILogic.empSP @ ?0 @ #) => (fun (x : function (CCall reify_imp_typ)) => Inj (typ := typ) (fEmp (func := func) x)).
-(*
-Reify Pattern patterns_java += (!! @Later.illater @ ?0 @ #) => (fun (x : function (CCall reify_imp_typ)) => (fLater (func := func) x)).
-*)
-
-Reify Pattern patterns_java += (!! method_spec) => (fMethodSpec).
-
-(** Program Logic **)
-
-
-Reify Pattern patterns_java += (!! triple) => (Inj (typ := typ) fTriple).
-Reify Pattern patterns_java += (!!method_lookup) => (Inj (typ := typ) fMethodLookup).
-Reify Pattern patterns_java += (!!field_lookup) => (Inj (typ := typ) fFieldLookup).
-Reify Pattern patterns_java += (!!m_ret) => (Inj (typ := typ) fMethodRet).
-Reify Pattern patterns_java += (!!m_body) => (Inj (typ := typ) fMethodBody).
-Reify Pattern patterns_java += (!!m_params) => (Inj (typ := typ) fMethodArgs).
-
-Reify Pattern patterns_java += (!! eval @ (RHasType dexpr (?0))) => (fun e : id dexpr => evalDExpr e).
-Reify Pattern patterns_java += (!! @stack_get @?0 @ ?1) => (fun _ _ : function (CCall reify_imp_typ) =>
-                                                              Inj (typ := typ) (fStackGet (typ := typ) (func := func))).
-Reify Pattern patterns_java += (!! stack_add (val := val)) => (Inj (typ := typ) (fStackSet (typ := typ) (func := func))).
-
-Reify Pattern patterns_java += (!! pointsto) => (Inj (typ := typ) fPointsto).
-Reify Pattern patterns_java += (!! prog_eq) => (Inj (typ := typ) fProgEq).
-Reify Pattern patterns_java += (!! typeof) => (Inj (typ := typ) fTypeOf).
-
-Reify Pattern patterns_java += (!! (@substl_trunc Lang.var val _)) => (Inj (typ := typ) (fTruncSubst (func := func) (typ := typ))).
-Reify Pattern patterns_java += (!! (@substl Lang.var val _)) => (Inj (typ := typ) (fSubst (func := func) (typ := typ))).
-
-Reify Pattern patterns_java += (!! @nil @ ?0) => (fun (x : function (CCall reify_imp_typ)) => (Inj (typ := typ) (fNil (func := func) x))).
-Reify Pattern patterns_java += (!! @cons @ ?0) => (fun (x : function (CCall reify_imp_typ)) => (Inj (typ := typ) (fCons (func := func) x))).
-(* Require Import MirrorCore.Lib.ListOpView.
-Reify Pattern patterns_java += (!! @length @ ?0) => (fun (x : function (CCall reify_imp_typ)) => (Inj (typ := typ) (fLength (func := func) x))).
-Reify Pattern patterns_java += (!! @combine @ ?0 @ ?1) => (fun (x y : function (CCall reify_imp_typ)) => (Inj (typ := typ) (fCombine (func := func) x y))).
-Reify Pattern patterns_java += (!! @map @ ?0 @ ?1) => (fun (x y : function (CCall reify_imp_typ)) => (Inj (typ := typ) (fMap (func := func) x y))).
-Reify Pattern patterns_java += (!! @fold_right @ ?0 @ ?1) => (fun (x y : function (CCall reify_imp_typ)) => (Inj (typ := typ) (fFold (func := func) x y))).
-*)
-
-Reify Pattern patterns_java += (!! (@apply_subst Lang.var val) @ ?0) => (fun (x : function (CCall reify_imp_typ)) => Inj (typ := typ) (fApplySubst (func := func) x)).
-Reify Pattern patterns_java += (!! @subst1 Lang.var val _) => (Inj (typ := typ) (fSingleSubst (func := func))).
-Reify Pattern patterns_java += (!! @field_lookup) => (Inj (typ := typ) fFieldLookup).
-(** Applicative **)
-Reify Pattern patterns_java += (!! @Applicative.ap @ !! (Fun Lang.stack) @ # @ ?0 @ ?1) => (fun (x y : function (CCall reify_imp_typ)) => Inj (typ := typ) (fAp (func := func) x y)).
-Reify Pattern patterns_java += (!! @Applicative.pure @ !! (Fun Lang.stack) @ # @ ?0) => (fun (x : function (CCall reify_imp_typ)) => Inj (typ := typ) (fPure (func := func) x)).
-
-Let elem_ctor : forall x : typ, typD x -> @SymEnv.function _ _ :=
-  @SymEnv.F _ _.
-
-Ltac reify_imp e :=
-  let k fs e :=
-      pose e in
-  reify_expr reify_imp k
-             [[ (fun (y : @mk_dvar_map _ _ _ _ term_table elem_ctor) => True) ]]
-             [[ e ]].
-
-
-Context {fs : Environment}.
-
-Goal (forall (Pr : Program) (C : class) (v : val) (x f : String.string) (fields : list field) (ex : @Open.expr Lang.var val), True).
-  intros Pr C v x f fields ex.
-  reify_imp (typeof C v).
-  reify_imp (field_lookup).
-  reify_imp (field_lookup Pr C fields).
-
-  pose ((fun (_ : @Stack.stack Lang.var val) => null) : @Open.expr Lang.var val) as e2.
-  pose ((fun (_ : Lang.stack) => null) : Lang.stack -> val) as e3.
-
-  reify_imp (pure (T := Fun Lang.stack) pointsto).
-
-  reify_imp (pure (T := Fun Lang.stack) pointsto).
-
-  reify_imp (fun a b c => pointsto a b c).
-
-  reify_imp e2.
-
-  reify_imp e3.
-
-  reify_imp (ap (T := Fun Lang.stack) (ap (T := Fun Lang.stack) (pure (@eq val)) e2) e2).
-
-  pose (E_val (vint 3)) as d.
-
-  reify_imp ((ap (ap (T := Fun Lang.stack) (pure (@eq val)) (eval d)) (pure (vbool true)))).
-
-  generalize String.EmptyString. intro c.
-  reify_imp (cread c c c).
-
-   reify_imp (ltrue |-- {[ ltrue ]} cread c c c {[ ltrue ]}).
-
-  reify_imp cskip.
-
-  reify_imp (forall P, P /\ P).
-
-  reify_imp (forall x : nat, x = x).
-  reify_imp (exists x : nat, x = x).
-
-  reify_imp (@subst1 Lang.var val _).
-  reify_imp (cseq cskip cskip).
-
-  reify_imp (@map nat nat).
-  reify_imp (ILogic.lentails True True).
-
-  reify_imp ((True -> False) -> True).
-  reify_imp (forall P Q, P /\ Q).
-
-  reify_imp (forall P : sasn, ILogic.lentails ILogic.ltrue P).
-  reify_imp (forall (G : spec) (P Q : sasn), ILogic.lentails G (triple P Q cskip)).
-  generalize (String.EmptyString : String.string).
-  intro y.
-
-  reify_imp (stack_get (A := Lang.var) (val := val)).
-  reify_imp (@stack_get Lang.var val y).
-
-  reify_imp (stack_get (val := val) y).
-
-  reify_imp (y = y).
-
-  reify_imp (@ltrue sasn _).
-
-  exact I.
-
-Defined.
-
-Ltac reify_aux e n :=
-  let k fs e :=
-      pose e as n in
-  reify_expr reify_imp k
-             [[ (fun (y : @mk_dvar_map _ _ _ _ term_table elem_ctor) => True) ]]
-             [[ e ]].
